Added basis definition, inductive predicate definition, and induction theorem.

States.v
@@ -1,6 +1,7 @@
 Require Import New.Complex.
 Require Import New.Field.
 Require Import Scalars.
+Require Import Coq.Sets.Ensembles.
 
 (* Fundamental operations on states. *)
 Class StateOps Scalar State
@@ -20,3 +21,137 @@ Class States Scalar State
   {state_ops : StateOps Scalar State} := {
   complex_st :> Complex State
 }.
+
+(* Is a set of states B a basis for state S, the inductive version *)
+Inductive state_basis
+  {Scalar} {State}
+  {sops : ScalarOps Scalar}
+  {state_ops : StateOps Scalar State}
+  (B : Ensemble State) :
+  State -> Prop :=
+  (* Everything is a basis for null *)
+  | state_null : state_basis B null
+  (* B is a basis for S if it contains S *)
+  | state_in_basis : forall (S : State),
+                       In State B S -> state_basis B S
+  (* B is a basis for a join if it's a basis for the components *)
+  | state_join_basis : forall (S1 S2 : State),
+                         state_basis B S1 ->
+                         state_basis B S2 ->
+                         state_basis B (join S1 S2)
+  (* B is a basis for a meet if it's a basis for the components *)
+  | state_meet_basis : forall (S1 S2 : State),
+                              state_basis B S1 ->
+                              state_basis B S2 ->
+                              state_basis B (meet S1 S2)
+  (* B is a basis for a scalar product if it's a basis for the inner state *)
+  | state_scalar_basis : forall (a : Scalar) (S : State),
+                                state_basis B S ->
+                                state_basis B (scalar_prod a S)
+  (* B is a basis for a complex conjugate if it's a basis for the inner state *)
+  | state_conj_basis : forall (S : State),
+                              state_basis B S ->
+                              state_basis B (~ S).
+
+(* Inductive predicates on states.  Basically, predicates that behave
+ * nicely in induction. *)
+Definition state_pred_inductive
+  {Scalar} {State}
+  {sops : ScalarOps Scalar}
+  {state_ops : StateOps Scalar State}
+  (B : Ensemble State) (P : State -> Prop) : Prop :=
+  (forall (S : State), In State B S -> P S) /\
+  (forall (S1 S2 : State), P S1 -> P S2 -> P (join S1 S2)) /\
+  (forall (S1 S2 : State), P S1 -> P S2 -> P (meet S1 S2)) /\
+  (forall (S : State) (a : Scalar), P S -> P (scalar_prod a S)) /\
+  (forall (S : State), P S -> P (~ S)) /\
+  P null.
+
+(* Helper used in proof of the induction principle over a basis. *)
+Definition P_if_basis
+  {Scalar} {State}
+  {sops : ScalarOps Scalar}
+  {state_ops : StateOps Scalar State}
+  (P : State -> Prop) (B : Ensemble State) (S : State) :=
+  state_basis B S -> P S.
+
+(* Induction theorem with basis sets.  Any inductive predicate P over
+ * a basis B holds for all elements of any state S such that B is a
+ * basis for S.
+ *)
+Theorem state_basis_induction
+  {Scalar} {State}
+  {sops : ScalarOps Scalar}
+  {state_ops : StateOps Scalar State}
+  (B : Ensemble State) (P : State -> Prop) :
+  state_pred_inductive B P -> (forall (S : State), state_basis B S -> P S).
+Proof.
+  unfold state_pred_inductive.
+  intros (basis_P & join_P & meet_P & scalar_P & conj_P & null_P).
+  intros.
+  cut (state_basis B S).
+  revert H.
+  replace (state_basis B S -> P S) with (P_if_basis P B S).
+  apply (state_basis_ind Scalar State sops state_ops B).
+  unfold P_if_basis.
+  intro.
+  assumption.
+  intros.
+  unfold P_if_basis.
+  intro.
+  apply basis_P.
+  assumption.
+  unfold P_if_basis.
+  intros.
+  apply join_P.
+  apply H0.
+  assumption.
+  apply H2.
+  assumption.
+  unfold P_if_basis.
+  intros.
+  apply meet_P.
+  apply H0.
+  assumption.
+  apply H2.
+  assumption.
+  unfold P_if_basis.
+  intros.
+  apply scalar_P.
+  apply H0.
+  assumption.
+  unfold P_if_basis.
+  intros.
+  apply conj_P.
+  apply H0.
+  assumption.
+  unfold P_if_basis.
+  reflexivity.
+  assumption.
+Qed.
+
+(* Is B a basis for all states in set SS? *)
+Definition state_set_basis
+  {Scalar} {State}
+  {sops : ScalarOps Scalar}
+  {state_ops : StateOps Scalar State}
+  (B : Ensemble State) (SS : Ensemble State) :=
+  forall (S : State), In State SS S -> state_basis B S.
+
+(* A version of the basis induction theorem for sets of states. *)
+Lemma state_set_basis_induction
+  {Scalar} {State}
+  {sops : ScalarOps Scalar}
+  {state_ops : StateOps Scalar State}
+  (B : Ensemble State) (SS : Ensemble State) (P : State -> Prop) :
+  state_pred_inductive B P -> state_set_basis B SS ->
+  (forall (S : State), In State SS S -> P S).
+Proof.
+  intro.
+  unfold state_set_basis.
+  intros.
+  apply H0 in H1.
+  apply (state_basis_induction B).
+  assumption.
+  assumption.
+Qed.
